state randomized testing soundness

Veil/DSL/Random/Main.lean
@@ -4,6 +4,7 @@ import Veil.Util.Meta
 import Veil.Util.DSL
 import Veil.Model.TransitionSystem
 import Veil.DSL.Specification.SpecDef
+import Plausible
 
 open Lean Lean.Elab.Command Lean.Meta Lean.Elab.Term
 
@@ -40,3 +41,52 @@ def deriveGen (inductiveTypeStx : Term) : TermElabM Syntax := do
 elab "#deriveGen" t:term : command => do
   let stx <- runTermElabM (fun _ => deriveGen t)
   elabCommand stx
+
+open Plausible
+
+variable [sys : RelationalTransitionSystem ρ σ]
+variable {labType : Type} (genL : Gen labType)
+variable (nextComp : labType -> VeilExecM .external ρ σ Unit)
+variable (next_refine : ∀ (rd : ρ) (st st' : σ) (l : labType),
+  (nextComp l).operational rd st st' (Except.ok ()) ->
+  sys.next rd st st')
+variable (r₀ : ρ) (s₀ : σ) (hinit : sys.init r₀ s₀)
+
+#check Random Id labType
+
+def random_transition (s : σ) : Gen (DivM (Except ExId σ)) := do
+  let l <- genL
+  return match nextComp l |>.run r₀ s with
+    | .res (.ok ⟨_, s'⟩) => .res (.ok s')
+    | .res (.error e) => .res (.error e)
+    | .div => .div
+
+structure RandomTrace (σ : Type) where
+  trace : Array σ
+  thrownException? : Option ExId
+  numberOfSteps : Nat
+  safe? : Bool
+
+def check_safety (steps : Nat) (cfg : Configuration) [∀ r s, Testable (sys.safe r s)] : Gen (RandomTrace σ) := do
+  let mut trace := #[]
+  let mut s := s₀
+  let mut numberOfSteps := 0
+  for _ in [0:steps] do
+    let step ← random_transition genL nextComp r₀ s
+    match step with
+    | .res (.ok s') =>
+      match <- Testable.runProp (sys.safe r₀ s') cfg true with
+      | .success _ | .gaveUp _ =>
+        s := s'
+        trace := trace.push s
+        numberOfSteps := numberOfSteps + 1
+      | .failure _ _ _ =>
+        return ⟨trace, .none, numberOfSteps, false⟩
+    | .res (.error e) =>
+      return ⟨trace, .some e, numberOfSteps, false⟩
+    | .div => pure ()
+  return ⟨trace, .none, numberOfSteps, true⟩
+
+lemma check_safety_sound (size : Nat) (steps : Nat) (cfg : Configuration) [∀ r s, Testable (sys.safe r s)] :
+  (ReaderT.run (check_safety genL nextComp r₀ s₀ steps cfg) ⟨size⟩ |>.run seed).1.safe? = false ->
+  ¬ sys.isInvariant sys.safe := by sorry
